---
jupytext:
  formats: ipynb,md:myst
  text_representation:
    extension: .md
    format_name: myst
    format_version: 0.13
    jupytext_version: 1.10.3
kernelspec:
  display_name: Python 3.9.4 64-bit
  language: python
  name: python394jvsc74a57bd0085761d8a84a55f3b91b6696b289e6480df59aded311489218ab7e58f5e20cd3
---
# Basic Rules of Differentiation

## The Rules

```{admonition} Derivative of a Constant
:class: info
For any real number $c$, 

$$
\frac{d}{dx}(c) = 0
$$
```

```{admonition} The Power Rule
:class: info

For any real number $n$, 

$$
\frac{d}{dx}(x^n) = nx^{n-1}
$$
```

```{admonition} Derivative of a Constant Multiple of a Function
:class: info

For any real number $c$, 

$$
\frac{d}{dx}[cf(x)] = c\frac{d}{dx}[f(x)]
$$
```

```{admonition} The Sum/Difference Rule
:class: info

$$
\frac{d}{dx}[f(x)\pm g(x)] = \frac{d}{dx}[f(x)]\pm \frac{d}{dx}[g(x)]
$$
```

````{admonition} The Product Rule
:class: info

$$
\frac{d}{dx}[f(x)g(x)] = f'(x)g(x) + f(x)g'(x)
$$

```{admonition} Tutor Talk
:class: tip

If $y=(1^{st})(2^{nd})$, then 

$$y'=(d1^{st})(2^{nd}) + (1^{st})(d2^{nd}).$$
```
````

````{admonition} The Quotient Rule
:class: info

If $g(x)\neq 0$, 

$$
\frac{d}{dx}\left[\frac{f(x)}{g(x)}\right] = \frac{f'(x)g(x) - f(x)g'(x)}{[g(x)]^2}
$$

```{admonition} Tutor Talk
:class: tip

If $y=\frac{Hi}{Lo}$, 

$$y' = \frac{(Lo)(dHi) - (Hi)(dLo)}{LoLo}.$$
```
````

```{admonition} The Chain Rule
:class: info

$$
\frac{d}{dx}\left[g(f(x))\right] = g'(f(x))f'(x)
$$
```

```{admonition} The General Power Rule
:class: info

$$
\frac{d}{dx}[f(x)]^n = n[f(x)]^{n-1}f'(x)
$$

This is a special case of the Chain Rule with $g(x) = x^n$.
```



## Applying the Rules


### Example 1 (Sum and Constant Multiple Rule)

Find the derivative of the function 

$$f(x) = 5x^2 - 4x + 2 + \frac{3}{x^4}$$ 

using the basic rules of differentiation.


```{admonition} Step 1: Remember the sum rule.
:class: tip, dropdown

Since $f(x)$ is the sum of functions, remember the sum rule for derivatives.

$$
\frac{d}{dx}[f(x)\pm g(x)] = \frac{d}{dx}[f(x)]\pm \frac{d}{dx}[g(x)]
$$
```

```{admonition} Step 2: Apply the sum rule.
:class: tip, dropdown

\begin{align*}
f'(x)
&= \frac{d}{dx}\left(5x^2-4x+2 +\frac{3}{x^4}\right) \\
&=\frac{d}{dx}\left(5x^2\right)-\frac{d}{dx}\left(4x^1\right)+\frac{d}{dx}\left(2\right)+\frac{d}{dx}\left(3x^{-4}\right)
\end{align*}
```


```{admonition} Step 3: Remember the constant multiple rule.
:class: tip, dropdown

Since several terms of $f(x)$ are a constant times a function, remember the constant multiple rule for derivatives.

$$
\frac{d}{dx}[cf(x)] = c\frac{d}{dx}[f(x)]
$$
```

```{admonition} Step 4: Apply the constant multiple rule.
:class: tip, dropdown

\begin{align*}
f'(x)
&= 5\frac{d}{dx}\left(x^2\right) - 4\frac{d}{dx}\left(x^1\right) + \frac{d}{dx}\left(2\right) + 3\frac{d}{dx}\left(x^{-4}\right)
\end{align*}
```

```{admonition} Step 5: Compute the derivative of each term.
:class: tip, dropdown

Remember $x^0=1$.

\begin{align*}
f'(x) 
&= 5\frac{d}{dx}\left(x^2\right)-4\frac{d}{dx}\left(x^1\right)+0+3\frac{d}{dx}\left(x^{-4}\right) && \hbox{$\dfrac{d}{dx}(c) = 0$ for any constant $c$}\\ \\ 
&= 5 \cdot 2x^{2-1} -  4\cdot1x^{1-1} + 3\cdot (-4)x^{-4-1} && \hbox{Power Rule, $\dfrac{d}{dx}x^n = nx^{n-1}$}\\ \\
&= 10x^1 - 4x^0 - 12x^{-5} && \hbox{Simplify}\\
%&= 10x - 4 - \frac{12}{x^5}
\end{align*}

Therefore,

$$f'(x) = 10x - 4 - \frac{12}{x^5}$$
```



### Example 2 (Product Rule)

Find the derivative of the function 

$$h(x)=(3x^2+1)(x^2+x+1)$$ 

using the basic rules of differentiation.


```{admonition} Step 1: Remember the product rule.
:class: tip, dropdown

Since $h(x)$ is the product of two functions, remember the product rule for derivatives.

$$
\frac{d}{dx}[f(x)g(x)]=f'(x)g(x)+f(x)g'(x)
$$
```

```{admonition} Step 2: Identify the two functions being multiplied.
:class: tip, dropdown

$$ f(x)=3x^2+1 ~~~\text{  and  }~~~ g(x)=x^2+x+1$$
```

```{admonition} Step 3: Compute the derivative of each function.
:class: tip, dropdown

\begin{align*}
f'(x) 
&= \frac{d}{dx}(3x^2 + 1) \\
&= \frac{d}{dx}(3x^2) + \frac{d}{dx}(1) && \hbox{Sum Rule}\\
&= 3\cdot 2x + 0 && \hbox{Power Rule & $\dfrac{d}{dx}(c) = 0$} \\
&= 6x \\ \\
g'(x) 
&= \frac{d}{dx}(x^2+x+1)\\
&= \frac{d}{dx}(x^2) + \frac{d}{dx}(x) + \frac{d}{dx}(1) && \hbox{Sum Rule}\\
&= 2x + 1 + 0 && \hbox{Power Rule & $\dfrac{d}{dx}(c) = 0$} \\
&= 2x + 1
\end{align*}
```

```{admonition} Step 4: Compute $h'(x)$.
:class: tip, dropdown

\begin{align*}
h'(x) &= f'(x)g(x)+f(x)g'(x) && \hbox{Product Rule}\\ \\
&= (6x)(x^2+x+1) + (3x^2+1)(2x+1) && \hbox{Using Steps 2 & 3}\\ \\
&= 6x^3+6x^2+6x+6x^3+3x^2+2x+1 && \hbox{Expand}\\ \\
&=12x^3+9x^2+8x+1 && \hbox{Combine like terms}
\end{align*}
```


### Example 3 (Quotient Rule)

Find the derivative of the function 

$$h(x)=\dfrac{x^3-7x+10}{x^2+4}$$ 

using the basic rules of differentiation and then evaluate $h'(2)$.

```{admonition} Step 1: Remember the quotient rule.
:class: tip, dropdown

Since $h(x)$ is the quotient of two functions, remember the quotient rule for derivatives.

$$
\frac{d}{dx}\left[\frac{f(x)}{g(x)}\right]=\frac{f'(x)g(x)-f(x)g'(x)}{[g(x)]^2}
$$
```

```{admonition} Step 2: Apply the quotient rule to the given function.
:class: tip, dropdown

\begin{align*}
h'(x)
& =\frac{\left[\frac{d}{dx}(x^3-7x+10)\right](x^2+4)-(x^3-7x+10)\left[\frac{d}{dx}(x^2+4)\right]}{(x^2+4)^2} \\ 
&= \frac{(3x^2-7)(x^2+4)-(x^3-7x+10)(2x)}{(x^2+4)^2} 
\end{align*}
```


```{admonition} Step 3: Simplify.
:class: tip, dropdown

\begin{align*}
h'(x)
&=\frac{(3x^4+5x^2-28)-(2x^4-14x^2+20x)}{(x^2+4)^2} && \hbox{Expand numerator}\\ 
&=\frac{x^4+19x^2-20x-28}{(x^2+4)^2} && \hbox{Combine like terms}
\end{align*}
```

```{admonition} Step 4: Simplify.
:class: tip, dropdown

Evaluate $h'(2)$.

\begin{align*}
h'(2) &= \frac{2^4+19\cdot2^2-20\cdot2-28}{(2^2+4)^2}\\ \\
&=\frac{16+19\cdot 4-20\cdot 2-28}{(4+4)^2}\\ \\
&=\frac{16+76-40-28}{8^2}\\ \\
&=\frac{24}{64}\\ \\
&=\frac{3}{8}
\end{align*}
```

```{admonition} Good to know
:class: warning

Keep in mind that if the only goal is to compute $h'(2)$, then Step 3 can be skipped and $x=2$ can be plugged in immediately after computing the derivative in Step 2.  This will reduce the number of computations and help avoid some possible algebraic mistakes while simplifying.
```


### Example 4 (General Power Rule)

Find the derivative of the function 

$$h(x) = \sqrt{3x^2 - 4x + 2}$$ 

using the basic rules of differentiation.

```{admonition} Step 1: Remember the general power rule.
:class: tip, dropdown

Since $h(x)$ can be rewritten as $(3x^2 - 4x + 2)^{1/2}$, remember the general power rule.

$$
\frac{d}{dx}[f(x)]^n = n[f(x)]^{n-1}f'(x)
$$
```

```{admonition} Step 2: Apply the rule and simplify.
:class: tip, dropdown

Apply the general power rule with $n=1/2$ and $f(x) = 3x^2 - 4x + 2$ and then simplify.

\begin{align*}
h'(x) &= \frac{d}{dx} (3x^2 - 4x + 2)^{1/2}\\ \\
&= \frac{1}{2}(3x^2 - 4x + 2)^{1/2 - 1}  \frac{d}{dx}(3x^2 - 4x + 2) && \hbox{General Power Rule}\\ \\
&= \frac{1}{2}(3x^2 - 4x + 2)^{-1/2}  (3\cdot 2x^{2-1} - 4x^{1-1} + 0)\\ \\
&= \frac{1}{2}(3x^2 - 4x + 2)^{-1/2}  (6x - 4)\\ \\
&= \frac{2(3x-2)}{2(3x^2-4+2)^{1/2}} &&\hbox{Simplify}\\ \\
&= \frac{3x-2}{\sqrt{3x^2-4+2}}
\end{align*}
```


### Example 5 (Product and General Power Rule)

Find the derivative of the function 

$$h(x) = (4x+1)^3(2x-5)^4$$ 

using the basic rules of differentiation.


```{admonition} Step 1: Remember the product rule.
:class: tip, dropdown

Since $h(x)$ is the product of two functions, remember the product rule for derivatives.

$$
\frac{d}{dx}[f(x)g(x)]=f'(x)g(x)+f(x)g'(x)
$$
```

```{admonition} Step 2: Apply the product rule.
:class: tip, dropdown

Apply the product rule with $f(x) = (4x+1)^3$ and $g(x) = (2x-5)^4$.

\begin{align*}
h'(x) 
&= \left[\frac{d}{dx}(4x+1)^3\right](2x-5)^4 + (4x+1)^3\left[\frac{d}{dx}(2x-5)^4\right]\\ \\
&= \left[3(4x+1)^2\cdot 4\right](2x-5)^4 + (4x+1)^3\left[4(2x-5)^3\cdot 2\right] 
\end{align*}

Notice how the general power rule was used to compute the derivative of both $(4x+1)^3$ and $(2x-5)^4$.
```

```{admonition} Step 3: Pull out common factors.
:class: tip, dropdown

\begin{align*}
h'(x) &= 4(4x+1)^2(2x-5)^3\left[3(2x-5) + 2(4x+1)\right]
\end{align*}
```

```{admonition} Step 4: Simplify.
:class: tip, dropdown

\begin{align*}
h'(x) &= 4(4x+1)^2(2x-5)^3\left[6x-15 + 8x+2\right]\\ \\
&= 4(4x+1)^2(2x-5)^3(14x-13)
\end{align*}
```



### Example 6 (Quotient and General Power Rule)

Find the derivative of the function 

$$h(x) = \dfrac{x^5}{(4x-7)^3}$$ 

using the basic rules of differentiation.


```{admonition} Step 1: Remember the quotient rule.
:class: tip, dropdown

Since $h(x)$ is the quotient of two functions, remember the quotient rule for derivatives.

$$
\frac{d}{dx}\left[\frac{f(x)}{g(x)}\right]=\frac{f'(x)g(x)-f(x)g'(x)}{[g(x)]^2}
$$
```

```{admonition} Step 2: Apply the quotient rule.
:class: tip, dropdown

Apply the quotient rule with $f(x) = x^5$ and $g(x) = (4x-7)^3$.

\begin{align*}
h'(x) 
&= \frac{\left[\frac{d}{dx}x^5\right](4x-7)^3 - x^5 \left[\frac{d}{dx}(4x-7)^3\right]}{[(4x-7)^3]^2} \\ \\
&= \frac{\left[5x^4\right](4x-7)^3 - x^5 \left[3(4x-7)^2 4\right]}{[(4x-7)^3]^2} && \hbox{Power Rule \& General Power Rule}\\ \\
&= \frac{5x^4(4x-7)^3 - 12x^5 (4x-7)^2}{(4x-7)^6}  && \hbox{Simplify}
\end{align*}
```

```{admonition} Step 3: Pull out common factors from the numerator.
:class: tip, dropdown

\begin{align*}
h'(x) &= \frac{x^4(4x-7)^2[5(4x-7) - 12x ]}{(4x-7)^6} 
\end{align*}
```

```{admonition} Step 4: Simplify.
:class: tip, dropdown

\begin{align*}
h'(x) &= \frac{x^4\cancel{(4x-7)^2}[20x-35 - 12x]}{(4x-7)^{\cancel{6}4}} \\ \\
&= \frac{x^4(8x-35)}{(4x-7)^4} 
\end{align*}
```

