{
 "cells": [
  {
   "cell_type": "markdown",
   "id": "008f1f29",
   "metadata": {},
   "source": [
    "# Examples: Computing Limits Algebraically\n",
    "\n",
    "## Example: Constant Function\n",
    "\n",
    "If $f(x) = 2$, find $\\lim\\limits_{x\\to 1^{-}}f(x)$.\n",
    "\n",
    "```{admonition} Solution\n",
    ":class: tip, dropdown\n",
    "\n",
    "$f$ is a constant function, hence a polynomial. Therefore, by Property 7 of {ref}`lim:prop_lim`, $\\lim\\limits_{x\\to 1} f(x) = f(1) = 2$. Since the limit exists, the one-sided limits exist, too and coincide with the limit. Thus, $\\lim\\limits_{x\\to 1^{-}}f(x) = 2$.\n",
    "```\n",
    "\n",
    "## Example: Rational Function (1)\n",
    "\n",
    "Evaluate \n",
    "\n",
    "$$\\lim\\limits_{x\\to -1} \\dfrac{x^3 +4x^2-x-3}{2x^2+1}.$$\n",
    "\n",
    "```{admonition} Solution\n",
    ":class: tip, dropdown\n",
    "\n",
    "The function \n",
    "\n",
    "$$ g(x) = \\dfrac{x^3 +4x^2-x-3}{2x^2+1}$$\n",
    "\n",
    "is a rational function, and since $2(-1)^2 + 1 = 3 \\neq 0$, it follows that $-1$ is in the domain of $g$. \n",
    "Again by Property 7 of {ref}`lim:prop_lim`, $\\lim\\limits_{x\\to -1} g(x)$ exists and equals \n",
    "\n",
    "$$g(-1) = \\frac{(-1)^3 + 4(-1)^2 - (-1) -3}{2(-1)^2+1} = \\frac{1}{3}.$$\n",
    "```\n",
    "\n",
    "## Example: Rational Function (2)\n",
    "\n",
    "Evaluate \n",
    "\n",
    "$$\\lim\\limits_{x\\to 2} \\dfrac{x^2 +4x-1}{x-2}.$$\n",
    "\n",
    "```{admonition} Solution\n",
    ":class: tip, dropdown\n",
    "\n",
    "For $x=2$, the denominator of the expression above is zero, so we cannot apply Property 7 of {ref}`lim:prop_lim` in this case. We observe that, as $x$ gets closer to $2$, the values of the denominator get closer to $0$, while the values of the numerator approach $11$. \n",
    "\n",
    "Moreover, if we approach $2$ from the left, the values of $(x^2 +4x-1)/(x-2)$ will be negative and approach $-\\infty$, while if we approach from the right, the values are positive and approach $+\\infty$. \n",
    "\n",
    "Therefore, neither the left-hand limit nor the right-limit exists, and hence $\\lim\\limits_{x\\to 2} \\dfrac{x^2 +4x-1}{x-2}$ does not exist either. \n",
    "```\n",
    "\n",
    "## Example: Piecewise Polynomial Function\n",
    "\n",
    "Evaluate $\\displaystyle\\lim_{x\\to 6} h(x)$, where\n",
    "\n",
    "\\begin{equation*}\n",
    "h(x)=\n",
    "\\begin{cases} \n",
    "x^2-4x-12 & \\hbox{if } x<6 \\\\\n",
    "8 & \\hbox{if } x=6 \\\\\n",
    "x^2-5x-6 & \\hbox{if } x>6 \\\\  \n",
    "\\end{cases}\n",
    "\\end{equation*}\n",
    "\n",
    "```{dropdown} **Step 1:** Find the limit from the left.\n",
    "\n",
    "In this case, since we are approaching 6 from the left, we can assume that $x<6$, and therefore $h(x) = x^2-4x-12$.\n",
    "\\begin{align*}\n",
    "\\lim_{x\\to 6^{-}} h(x) \n",
    "&= \\lim_{x\\to 6^-} x^2-4x-12\\\\ \\\\\n",
    "&= 6^2-4(6)-12 && \\text{Plug in $x=6$ (Property 7)}\\\\ \\\\\n",
    "&= 36-24-12 && \\text{Simplify}\\\\ \\\\\n",
    "&= 0\n",
    "\\end{align*}\n",
    "```\n",
    "\n",
    "```{dropdown} **Step 2:** Find the limit from the right. \n",
    "\n",
    "In this case, since we are approaching 6 from the right, we can assume that $x>6$, and therefore $h(x) = x^2-5x-6$.\n",
    "\\begin{align*}\n",
    "\\lim_{x\\to 6^{+}} h(x) \n",
    "&= \\lim_{x\\to 6^+} x^2-5x-6\\\\ \\\\\n",
    "&= 6^2-5(6)-6  && \\text{Plug in $x=6$ (Property 7)}\\\\ \\\\\n",
    "&= 36-30-6 && \\text{Simplify}\\\\ \\\\\n",
    "&= 0\n",
    "\\end{align*}\n",
    "```\n",
    "\n",
    "```{dropdown} **Step 3:** Check to see if the two limits are equal.\n",
    "\n",
    "Since $\\displaystyle \\lim_{x\\to 6^-} h(x) = \\lim_{x\\to 6^+} h(x) = 0$, we conclude that the limit exists and\n",
    "\n",
    "$$\\lim_{x\\to 6} h(x) = 0.$$\n",
    "```\n",
    "\n",
    "```{warning} \n",
    "Keep in mind that just because $\\displaystyle\\lim_{x\\to 6} h(x) \\neq h(6) = 8$, this does not mean that the limit does not exist.\n",
    "```"
   ]
  }
 ],
 "metadata": {
  "jupytext": {
   "formats": "ipynb,md:myst",
   "text_representation": {
    "extension": ".md",
    "format_name": "myst",
    "format_version": 0.13,
    "jupytext_version": "1.10.3"
   }
  },
  "kernelspec": {
   "display_name": "Python 3.9.4 64-bit",
   "language": "python",
   "name": "python3"
  },
  "language_info": {
   "codemirror_mode": {
    "name": "ipython",
    "version": 3
   },
   "file_extension": ".py",
   "mimetype": "text/x-python",
   "name": "python",
   "nbconvert_exporter": "python",
   "pygments_lexer": "ipython3",
   "version": "3.9.4"
  },
  "source_map": [
   13
  ]
 },
 "nbformat": 4,
 "nbformat_minor": 5
}