{
 "cells": [
  {
   "cell_type": "markdown",
   "id": "56f7b2a1",
   "metadata": {},
   "source": [
    "# Laws of Exponential and Logarithmic Functions\n",
    "\n",
    "Let $a$ and $b$ be positive numbers and $x$ and $y$ be real numbers. Let $m$ and $n$ be positive numbers.\n",
    "\n",
    "::::{grid} 2\n",
    ":::{grid-item-card} Exponential\n",
    "- **Addition of Exponents Law**\n",
    "\n",
    "  $$b^x b^y = b^{x + y}$$\n",
    "\n",
    "- **Difference of Exponents Law**\n",
    "\n",
    "  $$\\frac{b^x}{b^y} = b^{x - y}$$\n",
    "\n",
    "- **Exponentiation Law**\n",
    "\n",
    "  $$\\left( b^x \\right)^y = b^{xy}$$\n",
    "\n",
    "- **Product Distribution Law**\n",
    "\n",
    "  $$(ab)^x = a^xb^x$$\n",
    "\n",
    "- **Fractional Distribution Law**\n",
    "\n",
    "  $$\\left(\\frac{a}{b}\\right)^x = \\frac{a^x}{b^x}$$\n",
    ":::\n",
    "\n",
    ":::{grid-item-card} Logarithmic\n",
    "- **Logarithmic Addition Law** \n",
    "  \n",
    "  $$\\log_{b}(mn) = \\log_b(m) + \\log_b(n)$$\n",
    "\n",
    "- **Logarithmic Subtraction Law**\n",
    "\n",
    "  $$\\log_{b}\\left( \\frac{m}{n} \\right) = \\log_b(m) - \\log_b(n)$$\n",
    "\n",
    "- **Logarithm of a Power**\n",
    "\n",
    "  $$\\log_b(m^n) = n \\log_b(m)$$\n",
    "\n",
    "- **Logarithm of 1**\n",
    "\n",
    "  $$\\log_b(1) = 0 ~~\\&~~ \\ln(1) = 0$$\n",
    "\n",
    "- **Logarithm of the Base**\n",
    "\n",
    "  $$\\log_b(b) = 1 ~~\\&~~ \\ln(e) = 1$$\n",
    ":::\n",
    "::::\n",
    "\n",
    "\n",
    "## Cancellation properties\n",
    "\n",
    "::::{grid} 2\n",
    ":::{grid-item-card} \n",
    "\n",
    "- For all $x>0$  \n",
    "  \n",
    "  $$e^{\\ln(x)} = x$$\n",
    ":::\n",
    "\n",
    ":::{grid-item-card} \n",
    "- For all $x$ \n",
    "\n",
    "  $$\\ln(e^x) = x$$\n",
    ":::\n",
    "::::\n",
    "\n",
    "\n",
    "## Derivatives\n",
    "\n",
    "::::{grid} 2\n",
    ":::{grid-item-card}\n",
    "\n",
    "- **Derivative of $e^x$**\n",
    "\n",
    "  $$\\frac{d}{dx}e^x = e^x$$\n",
    "\n",
    "- **Derivative of $e^{f(x)}$**\n",
    "\n",
    "  $$\\frac{d}{dx}e^{f(x)} = e^{f(x)} f'(x)$$\n",
    ":::\n",
    "\n",
    ":::{grid-item-card}\n",
    "- **Derivative of $\\ln(x)$**\n",
    "\n",
    "  $$\\frac{d}{dx}\\ln(x) = \\frac{1}{x}$$\n",
    "\n",
    "- **Derivative of $\\ln(f(x))$**\n",
    "\n",
    "  $$\\frac{d}{dx}\\ln(f(x)) = \\frac{1}{f(x)} f'(x)$$\n",
    "\n",
    ":::\n",
    "::::\n",
    "\n",
    "\n",
    "\n",
    "## Example 1\n",
    "\n",
    "Find all values of $x$ such that $\\displaystyle 4^{x-x^2} = \\frac{1}{16^x}$.\n",
    "\n",
    "```{dropdown} **Step 1:** Write both sides of the equation as a power of $4$.\n",
    ":color: light\n",
    ":animate: fade-in\n",
    "\n",
    "Since the left-hand side is already written as a power of $4$, focus on the right-hand side.\n",
    "\n",
    "\\begin{align*}\n",
    "  \\frac{1}{16^x} \n",
    "  &= 16^{-x} \\\\\n",
    "  &= (4^2)^{-x}  && \\hbox{since $16 = 4^2$}\\\\\n",
    "  &= 4^{-2x} && \\hbox{since $(b^x)^y = b^{xy}$}\n",
    "\\end{align*}\n",
    "\n",
    "Therefore, the original equation can be rewritten in the following manner:\n",
    "\n",
    "$$4^{x-x^2} = 4^{-2x}.$$\n",
    "```\n",
    "\n",
    "\n",
    "```{dropdown} **Step 2:** Set the exponents equal to each other, and solve for $x$.\n",
    ":color: light\n",
    ":animate: fade-in\n",
    "\n",
    "\\begin{align*}\n",
    "  x-x^2 &= -2x && \\\\\n",
    "  3x-x^2 &= 0 && \\text{Move all variables to one side}\\\\\n",
    "  x(3-x) &= 0 && \\text{Factor}\\\\\n",
    "  x = 0&, x = 3 && \\text{Solve for } x \\text{ by setting each factor equal to } 0\n",
    "\\end{align*}\n",
    "```\n",
    "\n",
    "## Example 2\n",
    "\n",
    "Find all values of $x$ such that: \n",
    "\n",
    "$$2^{2x}-40\\cdot 2^x +256 = 0.$$\n",
    "\n",
    "```{dropdown} **Step 1:** Rewrite the equation in terms of $\\displaystyle 2^x$.\n",
    ":color: light\n",
    ":animate: fade-in\n",
    "\n",
    "$$(2^x)^2 -40\\cdot 2^x+256 = 0.$$\n",
    "```\n",
    "\n",
    "```{dropdown} **Step 2:** Let $\\displaystyle u = 2^x$.\n",
    ":color: light\n",
    ":animate: fade-in\n",
    "\n",
    "$$u^2-40u+256 =0.$$\n",
    "```\n",
    "\n",
    "```{dropdown} **Step 3:** Factor and solve for $u$.\n",
    ":color: light\n",
    ":animate: fade-in\n",
    "\n",
    "$$(u-8)(u-32) = 0.$$\n",
    "\n",
    "$$u=8 ~~~~ \\hbox{ or } ~~~~ u=32.$$\n",
    "```\n",
    "\n",
    "```{dropdown} **Step 4:** Substitute $2^x$ back in for $u$ and solve for $x$.\n",
    ":color: light\n",
    ":animate: fade-in\n",
    "\n",
    "\\begin{align*}\n",
    "  2^x &= 8 & 2^x &= 32\\\\\n",
    "  x&=3 & x&=5\n",
    "\\end{align*}\n",
    "```\n",
    "\n",
    "## Example 3\n",
    "\n",
    "Find all values of $t$ such that $\\dfrac{360}{1+9e^{-2t}} = 90$.\n",
    "\n",
    "```{dropdown} **Step 1:** Isolate $e^{-2t}$ using the following steps.\n",
    ":color: light\n",
    ":animate: fade-in\n",
    "\n",
    "\\begin{align*}\n",
    "  360 &= 90(1+9e^{-2t}) && \\text{Multiply both sides by the denominator} \\\\ \\\\\n",
    "  4 &= 1+9e^{-2t} && \\text{Divide both sides by 90} &&\\\\ \\\\\n",
    "  3 &= 9e^{-2t} && \\text{Subtract 1 from both sides}&&\\\\ \\\\\n",
    "  1/3 &= e^{-2t} && \\text{Divide both sides by 9}&&\n",
    "\\end{align*}\n",
    "```\n",
    "\n",
    "```{dropdown} **Step 2:** Take the natural logarithm of both sides.\n",
    ":color: light\n",
    ":animate: fade-in\n",
    "\n",
    "\\begin{align*}\n",
    "  \\ln \\left(\\frac{1}{3} \\right) \n",
    "  &= \\ln(e^{-2t}) \\\\ \n",
    "  &= -2t && \\hbox{Cancellation property $\\ln(e^x) = x$}\n",
    "\\end{align*}\n",
    "```\n",
    "\n",
    "```{dropdown} **Step 3:** Solve for $t$.\n",
    ":color: light\n",
    ":animate: fade-in\n",
    "\n",
    "\\begin{align*}\n",
    "  t \n",
    "  &= -\\frac{1}{2}  \\ln \\left( \\frac{1}{3}\\right)\\\\\n",
    "  &= \\frac{1}{2}\\ln(3)  && \\hbox{since $\\ln(1/3) = \\ln(3^{-1}) = -\\ln(3)$}\n",
    "\\end{align*}\n",
    "```\n",
    "\n",
    "## Example 4\n",
    "\n",
    "Expand the following expression:\n",
    "\n",
    "$$\\ln \\left(\\frac{\\sqrt[3]{(x+1)^2}\\cdot e^{5x}}{x}\\right).$$\n",
    "\n",
    "```{dropdown} **Step 1:** Use the laws of logarithms to expand the given expression.\n",
    ":color: light\n",
    ":animate: fade-in\n",
    "\n",
    "\\begin{align*}\n",
    "  \\ln \\left(\\frac{\\sqrt[3]{(x+1)^2}\\cdot e^{5x}}{x}\\right) \n",
    "  &= \\ln(\\sqrt[3]{(x+1)^2}\\cdot e^{5x}) - \\ln(x) && \\hbox{using $\\ln(m/n) = \\ln(m) - \\ln(n)$} \\\\ \\\\\n",
    "  &= \\ln(\\sqrt[3]{(x+1)^2}) + \\ln(e^{5x}) - \\ln(x) && \\hbox{using $\\ln(mn) = \\ln(m) + \\ln(n)$}\\\\ \\\\\n",
    "  %&= \\ln((x+1)^{2/3}) + \\ln(e^{5x}) - \\ln(x)\\\\ \\\\\n",
    "  &= \\frac{2}{3} \\ln(x+1) + 5x \\ln(e) - \\ln(x) && \\hbox{using $\\ln(m^n) = n\\ln(m)$}\\\\ \\\\\n",
    "  &= \\frac{2}{3} \\ln(x+1) + 5x - \\ln(x) && \\hbox{using $\\ln(e) = 1$.}\n",
    "\\end{align*}\n",
    "```\n",
    "\n",
    "## Example 5\n",
    "\n",
    "Find the tangent line to $y=\\dfrac{e^{27x}}{x^9}$ at the point $(1,e^{27})$.\n",
    "\n",
    "```{dropdown} **Step 1:** Recall the point-slope equation of a line.\n",
    ":color: light\n",
    ":animate: fade-in\n",
    "\n",
    "Point-Slope: \n",
    "\n",
    "$$y-b = m(x-a),$$\n",
    "\n",
    "where $m$ is the slope of the line and $(a,b)$ is a point on the line.\n",
    "```\n",
    "\n",
    "```{dropdown} **Step 2:** Compute the slope of the line by using the derivative. \n",
    ":color: light\n",
    ":animate: fade-in\n",
    "\n",
    "Recall $\\dfrac{d}{dx}e^{f(x)} = e^{f(x)} f'(x)$.\n",
    "\n",
    "$$y' = \\frac{e^{27x}\\cdot 27 \\cdot x^9 - e^{27x}\\cdot 9x^8}{x^{18}}.$$\n",
    "\n",
    "Since the given point is $(1,e^{27})$, plug in $x=1$ into the derivative to find the slope of the tangent line.\n",
    "\n",
    "\\begin{align*}\n",
    "  m\n",
    "  &= y'(1) \\\\\n",
    "  &= \\frac{e^{27}\\cdot 27 - e^{27}\\cdot 9}{1}\\\\\n",
    "  &= 18e^{27}.\n",
    "\\end{align*}\n",
    "```\n",
    "\n",
    "```{dropdown} **Step 3:** Write down the equation of the tangent line.\n",
    ":color: light\n",
    ":animate: fade-in\n",
    "\n",
    "Since we were given the point $(1,e^{27})$ (i.e., $a=1$ and $b=e^{27}$) and we found the slope ($m=18e^{27}$), we can now write down the equation of the tangent line using the point-slope equation of a line. \n",
    "\n",
    "$$y-e^{27} = 18e^{27}(x-1).$$\n",
    "```\n",
    "\n",
    "\n",
    "## Example 6\n",
    "\n",
    "Suppose the unit selling price $p(x)$ and the quantity supplied $x$ of a certain product is given by \n",
    "\n",
    "$$p(x) = x^3e^{5x}+12.$$\n",
    "\n",
    "\n",
    "Find the marginal revenue function $R'(x)$.\n",
    "\n",
    "```{dropdown} **Step 1:** Find the revenue function, $R(x)$, using the formula $R(x) = x\\cdot p(x)$.\n",
    ":color: light\n",
    ":animate: fade-in\n",
    "\n",
    "$$R(x) = x^4e^{5x} +12x.$$\n",
    "```\n",
    "\n",
    "```{dropdown} **Step 2:** Compute the derivative of $R(x)$. \n",
    ":color: light\n",
    ":animate: fade-in\n",
    "\n",
    "Recall $\\dfrac{d}{dx}e^{f(x)} = e^{f(x)} f'(x)$.\n",
    "\n",
    "\\begin{align*}\n",
    "  R'(x) \n",
    "  &= 4x^3(e^{5x})+x^4(e^{5x}\\cdot 5) + 12 && \\text{using Product Rule}\\\\\n",
    "  &= x^3 e^{5x}(4+5x) + 12.\n",
    "\\end{align*}\n",
    "```\n",
    "\n",
    "## Example 7\n",
    "\n",
    "Compute the derivative of $f(x) = \\ln\\left(\\dfrac{\\sqrt{6x+1}}{5x}\\right)$.\n",
    "\n",
    "```{dropdown} **Step 1:** Expand $f(x)$ using laws of logarithms.\n",
    ":color: light\n",
    ":animate: fade-in\n",
    "\n",
    "\\begin{align*}\n",
    "  \\ln\\left(\\dfrac{\\sqrt{6x+1}}{5x}\\right)\n",
    "  &= \\ln(\\sqrt{6x+1}) - \\ln(5x) && \\hbox{since $\\ln(m/n) = \\ln(m) - \\ln(n)$} \\\\ \\\\\n",
    "  &= \\ln((6x+1)^{1/2}) - [\\ln(5) + \\ln(x)] && \\hbox{since $\\ln(mn) = \\ln(m) + \\ln(n)$} \\\\ \\\\\n",
    "  &= \\frac{1}{2}\\ln(6x+1) - \\ln(5) - \\ln(x) && \\hbox{since $\\ln(m^n) = n\\ln(m).$}\n",
    "\\end{align*}\n",
    "```\n",
    "\n",
    "```{dropdown} **Step 2:** Compute the derivative.  Recall $\\dfrac{d}{dx}\\ln(f(x)) = \\dfrac{1}{f(x)} f'(x)$.\n",
    ":color: light\n",
    ":animate: fade-in\n",
    "\n",
    "\\begin{align*}\n",
    "  \\frac{d}{dx}\\left(\\frac{1}{2}\\ln(6x+1) - \\ln(5) - \\ln(x)\\right)\n",
    "  &= \\frac{1}{2}\\cdot \\frac{1}{6x+1}\\cdot 6 - 0 - \\frac{1}{x} \\\\\n",
    "  &= \\frac{3}{6x+1} - \\frac{1}{x}.\n",
    "\\end{align*}\n",
    "```\n",
    "\n",
    "\n",
    "## Example 8\n",
    "\n",
    "Let $\\ln(xy)+y^7 = x^3 + 2x$. Find $\\dfrac{dy}{dx}$.\n",
    "\n",
    "```{dropdown} **Step 1:** Differentiate both sides using implicit differentiation.\n",
    ":color: light\n",
    ":animate: fade-in\n",
    "\n",
    "$$\\frac{1}{xy} (y +xy') + 7y^6y' = 3x^2+2.$$\n",
    "```\n",
    "\n",
    "```{dropdown} **Step 2:** Multiply both sides by $xy$.\n",
    ":color: light\n",
    ":animate: fade-in\n",
    "\n",
    "\\begin{align*}\n",
    "  xy\\left[ \\frac{1}{xy} (y +xy') + 7y^6y' \\right]\n",
    "  &= xy\\frac{1}{xy} (y +xy') + xy\\cdot 7y^6y' \\\\\n",
    "  &= (y+xy') + 7xy^7y'\\\\\n",
    "  \\\\\n",
    "  xy\\left[ 3x^2 + 2 \\right]\n",
    "  &= 3x^3y + 2xy.\n",
    "\\end{align*}\n",
    "\n",
    "Therefore, \n",
    "\n",
    "$$y+xy' + 7xy^7y' = 3x^3y + 2xy.$$\n",
    "```\n",
    "\n",
    "```{dropdown} **Step 3:** Rearrange terms so that any term with a factor of $y'$ is on the left-hand side of the equation and all other terms are on the right-hand side.\n",
    ":color: light\n",
    ":animate: fade-in\n",
    "\n",
    "$$xy' + 7xy^7y' = 3x^3y + 2xy - y.$$\n",
    "```\n",
    "\n",
    "```{dropdown} **Step 4:** Factor out $y'$ on the left-hand side.\n",
    ":color: light\n",
    ":animate: fade-in\n",
    "\n",
    "$$y'(x + 7xy^7) = 3x^3y + 2xy - y.$$\n",
    "```\n",
    "\n",
    "```{dropdown} **Step 5:** Solve for $y'$.\n",
    ":color: light\n",
    ":animate: fade-in\n",
    "\n",
    "$$y' = \\frac{3x^3y + 2xy - y}{x + 7xy^7}.$$\n",
    "```"
   ]
  }
 ],
 "metadata": {
  "jupytext": {
   "formats": "ipynb,md:myst",
   "text_representation": {
    "extension": ".md",
    "format_name": "myst",
    "format_version": 0.13,
    "jupytext_version": "1.10.3"
   }
  },
  "kernelspec": {
   "display_name": "Python 3.9.4 64-bit",
   "language": "python",
   "name": "python3"
  },
  "language_info": {
   "codemirror_mode": {
    "name": "ipython",
    "version": 3
   },
   "file_extension": ".py",
   "mimetype": "text/x-python",
   "name": "python",
   "nbconvert_exporter": "python",
   "pygments_lexer": "ipython3",
   "version": "3.10.6"
  },
  "source_map": [
   13
  ]
 },
 "nbformat": 4,
 "nbformat_minor": 5
}